better spec for length, and a different formulation of listptr

examples/seplogic/SL.Examples.fst
@@ -271,19 +271,20 @@ let cond_test (r1 r2:ref int) (x:int) (b:bool)
 
 #reset-options "--print_full_names --__no_positivity"
 
-noeq type listptr' =
-  | Null :listptr'
-  | Cell :head:int -> tail:listptr -> listptr'
+noeq type listcell =
+  | Cell :head:int -> tail:listptr -> listcell
 
-and listptr = ref listptr'
+and listptr = option (ref listcell)
 
 #reset-options "--print_full_names --__temp_fast_implicits"
 
 let rec valid (p:listptr) (repr:list int) (m:memory) :Tot Type0 (decreases repr) =
-  match repr with
-  | []    -> m == (p |> Null)
-  | hd::tl -> exists (tail:listptr) (m1:memory). defined ((p |> Cell hd tail) <*> m1) /\ m == ((p |> Cell hd tail) <*> m1) /\ valid tail tl m1
-
+  defined m /\
+  (match repr with
+   | []    -> None? p /\ m == emp
+   | hd::tl -> Some? p /\
+             (exists (tail:listptr) (m1:memory). m == (((Some?.v p) |> Cell hd tail) <*> m1) /\ valid tail tl m1))
+                                                      
 private let __exists_elim_as_forall2
   (#a:Type) (#b:Type) (#p: a -> b -> Type) (#phi:Type)
   (_:(exists x y. p x y)) (_:(squash (forall (x:a) (y:b). p x y ==> phi)))
@@ -319,35 +320,42 @@ private let __implies_intros_with_processing_exists_and_and () :Tac unit
 			                   (fun _ -> or_else (fun _ -> rewrite h) idtac)))
             (fun _ -> fail "done")
 
-#set-options "--z3rlimit 30"
-private let __elim_list_match0 (#a:Type) (l:list a) (phi:Type) (psi:a -> list a -> Type) (rest:list a -> Type)
-  :Lemma (requires (((l == [] /\ phi) ==> rest []) /\
-                    (forall hd tl. (l == Cons hd tl /\ psi hd tl) ==> rest (Cons hd tl))))
-         (ensures  ((match l with
-	             | []         -> phi
-		     | Cons hd tl -> psi hd tl) ==> rest l))
-  = ()
+(*
+ * AR: these two lemmas are useless because of no match-ing in the unifier
+ *)
+// #set-options "--z3rlimit 30"
+// private let __elim_list_match0 (#a:Type) (l:list a) (phi:Type) (psi:a -> list a -> Type) (rest:list a -> Type)
+//   :Lemma (requires (((l == [] /\ phi) ==> rest []) /\
+//                     (forall hd tl. (l == Cons hd tl /\ psi hd tl) ==> rest (Cons hd tl))))
+//          (ensures  ((match l with
+// 	             | []         -> phi
+// 		     | Cons hd tl -> psi hd tl) ==> rest l))
+//   = ()
 
-private let __list_match_elim_as_cases (#l:list int) (#phi:list int -> Type0) (#psi:list int -> int -> list int -> Type0) (#rest:list int -> Type0)
-  (_:(match l with
-      | []         -> phi l
-      | Cons hd tl -> psi l hd tl))
-  (_:squash (((l == [] /\ phi []) ==> rest []) /\
-             ((forall hd tl. (l == Cons hd tl /\ psi (Cons hd tl) hd tl) ==> rest (Cons hd tl)))))
-  :Lemma (rest l)
-  = ()
+// private let __list_match_elim_as_cases (#l:list int) (#phi:list int -> Type0) (#psi:list int -> int -> list int -> Type0) (#rest:list int -> Type0)
+//   (_:(match l with
+//       | []         -> phi l
+//       | Cons hd tl -> psi l hd tl))
+//   (_:squash (((l == [] /\ phi []) ==> rest []) /\
+//              ((forall hd tl. (l == Cons hd tl /\ psi (Cons hd tl) hd tl) ==> rest (Cons hd tl)))))
+//   :Lemma (rest l)
+//   = ()
 
-private let __elim_list_match (h:binder) :Tac unit
-  = let t = `__list_match_elim_as_cases in
-    apply_lemma (mk_e_app t [pack (Tv_Var (bv_of_binder h))])
-    //clear h
+// private let __elim_list_match (h:binder) :Tac unit
+//   = let t = `__list_match_elim_as_cases in
+//     apply_lemma (mk_e_app t [pack (Tv_Var (bv_of_binder h))])
+//     //clear h
 
-let __elim_valid_without_match (p:listptr) (repr:list int) (m:memory) (goal:listptr -> list int -> memory -> Type0)
-  :Lemma (requires ((valid p repr m) /\
-                    ((repr == [] /\ m == (p |> Null)) ==> goal p [] (p |> Null)) /\
-		    (forall hd tl. (repr == Cons hd tl /\ (exists tail m1.  defined ((p |> Cell hd tail) <*> m1)  /\
-		                                                  m == ((p |> Cell hd tail) <*> m1)    /\
-							          valid tail tl m1)) ==> goal p (Cons hd tl) m)))
+//i tried a style where i pass the proof of valid p repr m as a squashed term
+//but even then unification fails
+//currently all the arguments have to be provided explicitly
+let __elim_valid_without_match
+  (#p:listptr) (#repr:list int) (#m:memory) (#goal:listptr -> list int -> memory -> Type0)
+  :Lemma (requires (((repr == [] /\ p == None /\ m == emp) ==> goal None [] emp) /\
+                    (forall hd tl. (repr == hd::tl /\
+	                       Some? p       /\
+			       (exists tail m1. m == (((Some?.v p) |> Cell hd tail) <*> m1) /\ valid tail tl m1))
+		              ==> goal p (Cons hd tl) m)))
          (ensures  (goal p repr m))
   = admit ()
 
@@ -356,91 +364,83 @@ let lemma_frame_exact (phi:memory -> memory -> memory -> memory -> Type0) (h h':
          (ensures  (exists (h0 h1:memory). defined (h0 <*> h1) /\ (h <*> h') == (h0 <*> h1) /\ phi h h' h0 h1))
   = ()
 
-let rec length (l:listptr) (fl:list int)
-  = (let x = !l in
-     match x with
-     | Null       -> (0 <: STATE int (fun p h -> p 0 emp))
-     | Cell hd tl -> 1 + length tl (FStar.List.Tot.Base.tl fl))
+let rec length (l:listptr)
+  = (match l with
+     | None   -> (0 <: STATE int (fun p h -> p 0 emp))
+     | Some r ->
+       let Cell hd tl = !r in
+       1 + length tl)
 
-    <: STATE int (fun p m -> valid l fl m /\ (defined m /\ p (List.Tot.length fl) m))
+    <: STATE int (fun p m -> exists (fl:list int). valid l fl m /\ p (List.Tot.length fl) m)
 
-    by (fun () -> ignore (forall_intros ());
-	       let h = implies_intro () in __elim_and h;
-	       ignore (implies_intros ());
-	       apply_lemma (`__elim_valid_without_match);
-	       assumption (); assumption (); assumption ();
-	       apply_lemma (`split_lem);
-	       apply_lemma (`split_lem); smt ();
-	       let h = implies_intro () in __elim_and h;
-	       let h = implies_intro () in rewrite h;
-	       let h = implies_intro () in rewrite h;
-	       apply_lemma (`lemma_singleton_heap_rw);
-	       apply_lemma (`split_lem); smt ();
-	       apply_lemma (`lemma_inline_in_patterns_two);
-	       apply_lemma (`split_lem); smt ();
-	       apply_lemma (`split_lem);
-	       ignore (implies_intro ());
-	       apply_lemma (`lemma_frame_out_empty_left);
-	       apply_lemma (`split_lem); smt ();
-	       apply_lemma (`split_lem); smt ();
-	       apply_lemma (`split_lem); smt ();
-	       apply_lemma (`lemma_frame_out_empty_left);
-	       smt ();
-	       ignore (implies_intro ());
-	       smt ();
+    by (fun _ -> ignore (forall_intros ());
+              let h = implies_intro () in __elim_exists1 h;
+	      let h = implies_intro () in __elim_and h;
+	      ignore (implies_intro ());
+	      apply_lemma (`__elim_valid_without_match);  //this is fragile
+	      assumption (); assumption (); assumption ();
+	      split ();
+	      let h = implies_intro () in __elim_and h;
+	      let h = implies_intro () in __elim_and h;
+	      let h = implies_intro () in rewrite h; let h = implies_intro () in rewrite h;
+              let h = implies_intro () in rewrite h;
+	      ignore (implies_intro ());
+	      split ();
+	      ignore (implies_intro ());
+	      apply_lemma (`lemma_frame_out_empty_left);
+	      split (); smt ();
+	      ignore (implies_intro ());
+	      split (); smt (); split (); smt ();
+	      apply_lemma (`lemma_frame_out_empty_left);
+	      smt (); smt ();
 
-               //inductive case
-	       ignore (forall_intros ());
-	       let h = implies_intro () in __elim_and h;
-	       let h = implies_intro () in rewrite h;
-	       let h = implies_intro () in __elim_exists2 h;
-	       let h = implies_intro () in __elim_and h;
-	       let h = implies_intro () in __elim_and h;
-	       ignore (implies_intro ());
-	       let h = implies_intro () in rewrite h;
-	       ignore (implies_intro ());
-	       apply_lemma (`lemma_rw);
-	       apply_lemma (`split_lem); smt ();
-	       apply_lemma (`split_lem); smt ();
-	       apply_lemma (`lemma_inline_in_patterns_two);
-	       apply_lemma (`split_lem); smt ();
-	       apply_lemma (`split_lem);
-	       ignore (implies_intro ());
-	       smt ();
-	       ignore (implies_intro ());
-	       apply_lemma (`lemma_inline_in_patterns_two);
-	       apply_lemma (`split_lem); smt ();
-	       apply_lemma (`split_lem);
-	       ignore (implies_intro ());
-	       apply_lemma (`lemma_frame_out_empty_right);
-	       apply_lemma (`split_lem); smt ();
-	       ignore (forall_intros ()); ignore (implies_intro ());
-	       apply_lemma (`lemma_frame_out_empty_right);
-	       apply_lemma (`split_lem); smt ();
-	       apply_lemma (`lemma_frame_out_empty_left);
-	       apply_lemma (`split_lem); smt ();
-	       apply_lemma (`split_lem); smt ();
-	       ignore (forall_intro ());
-	       ignore (implies_intro ());
-	       ignore (forall_intro ());
-	       apply_lemma (`split_lem); smt ();
-	       apply_lemma (`lemma_rewrite_sep_assoc2);
-	       apply_lemma (`lemma_frame_exact);
-	       apply_lemma (`split_lem); smt ();
-	       ignore (implies_intro ());
-	       apply_lemma (`split_lem); smt ();
-	       apply_lemma (`split_lem); smt ();
-	       apply_lemma (`split_lem); smt ();
-	       apply_lemma (`split_lem); smt ();
-	       apply_lemma (`lemma_frame_out_empty_left);
-	       apply_lemma (`split_lem); smt ();
-	       ignore (forall_intro ()); ignore (implies_intro ());
-	       apply_lemma (`split_lem); smt ();
-	       apply_lemma (`split_lem); smt ();
-	       apply_lemma (`lemma_frame_out_empty_left);
-	       apply_lemma (`split_lem); smt ();
-	       apply_lemma (`split_lem); smt ();
-	       apply_lemma (`split_lem); smt ();
-	       apply_lemma (`lemma_frame_out_empty_left);
-	       smt ();
-	       smt ())
+              //inductive case
+	      let hd_binder = forall_intro () in
+	      let tl_binder = forall_intro () in
+	      let h = implies_intro () in __elim_and h;
+	      let h = implies_intro () in __elim_and h;
+	      let h = implies_intro () in rewrite h;
+	      ignore (implies_intro ());
+	      let h = implies_intro () in __elim_exists2 h;
+	      let h = implies_intro () in __elim_and h;
+	      let h = implies_intro () in rewrite h;
+	      ignore (implies_intros ());
+	      split (); smt ();
+
+              ignore (implies_intro ());
+	      apply_lemma (`lemma_inline_in_patterns_two);
+	      split (); smt ();
+	      split ();
+	      ignore (implies_intro ());
+	      apply_lemma (`lemma_frame_out_empty_right);
+	      split (); smt ();
+	      ignore (forall_intro ());
+	      let h = implies_intro () in rewrite h;
+	      norm [delta_only ["FStar.Pervasives.Native.__proj__Some__item__v"]];
+	      apply_lemma (`lemma_rw);
+	      split (); smt ();
+	      split (); smt ();
+	      apply_lemma (`lemma_frame_out_empty_right);
+	      split (); smt ();
+	      apply_lemma (`lemma_frame_out_empty_right);
+	      split (); smt ();
+	      ignore (forall_intros ()); ignore (implies_intro ());
+	      apply_lemma (`lemma_rewrite_sep_comm);
+	      apply_lemma (`lemma_frame_exact);
+	      split (); smt ();
+	      let w = let bv, _ = inspect_binder tl_binder in pack (Tv_Var bv) in
+	      witness w;
+	      split (); smt (); split (); smt ();
+	      apply_lemma (`lemma_frame_out_empty_left);
+	      split (); smt ();
+	      ignore (forall_intro ());
+	      ignore (implies_intro ());
+	      split (); smt (); split (); smt ();
+	      apply_lemma (`lemma_frame_out_empty_left);
+	      split (); smt (); split (); smt ();
+	      split (); smt (); split (); smt ();
+	      apply_lemma (`lemma_frame_out_empty_left);
+	      split (); smt (); split (); smt (); split (); smt ();
+	      apply_lemma (`lemma_frame_out_empty_left);
+	      smt ();
+	      smt ())
